src/ToCoq.cpp
@@ -32,6 +32,27 @@
 using namespace clang;
 using namespace fmt;
 
+template<typename CLOSURE>
+void
+with_open_file(const llvm::Optional<std::string> path, CLOSURE f /* void f(Formatter&) */) {
+    if (path.hasValue()) {
+        std::error_code ec;
+        llvm::raw_fd_ostream output(*path, ec);
+        if (ec.value()) {
+            llvm::errs() << *path << ": " << ec.message() << "\n";
+        } else {
+            Formatter fmt {output};
+            f(fmt);
+        }
+    }
+}
+
+void
+printDecl(const clang::Decl* decl, CoqPrinter& print, ClangPrinter& cprint) {
+    if (cprint.printDecl(decl, print))
+        print.cons();
+}
+
 void
 ToCoqConsumer::toCoqModule(clang::ASTContext *ctxt,
                            clang::TranslationUnitDecl *decl) {
@@ -48,85 +69,91 @@ ToCoqConsumer::toCoqModule(clang::ASTContext *ctxt,
 
     ::Module mod;
 
-    build_module(decl, mod, filter, specs, compiler_, elaborate_);
+    bool templates = templates_file_.hasValue();
+    build_module(decl, mod, filter, specs, compiler_, elaborate_, templates);
 
-    if (output_file_.hasValue()) {
-        std::error_code ec;
-        llvm::raw_fd_ostream code_output(*output_file_, ec);
-        if (ec.value()) {
-            llvm::errs() << "Failed to open generation file: " << *output_file_
-                         << "\n"
-                         << ec.message() << "\n";
+    with_open_file(output_file_, [this, &ctxt, &mod](Formatter& fmt){
+        CoqPrinter print(fmt, false);
+        ClangPrinter cprint(compiler_, ctxt);
+
+        fmt << "Require Import bedrock.lang.cpp.parser." << fmt::line
+            << fmt::line << "#[local] Open Scope bs_scope." << fmt::line;
+        // << "Import ListNotations." << fmt::line;
+
+        fmt << fmt::line
+            << "Definition module : translation_unit := " << fmt::indent
+            << fmt::line << "Eval reduce_translation_unit in decls"
+            << fmt::nbsp;
+
+        print.begin_list();
+        for (auto decl : mod.declarations()) {
+            printDecl(decl, print, cprint);
+        }
+        for (auto decl : mod.definitions()) {
+            printDecl(decl, print, cprint);
+        }
+        for (auto decl : mod.asserts()) {
+            printDecl(decl, print, cprint);
+        }
+        print.end_list();
+        print.output() << fmt::nbsp;
+        if (ctxt->getTargetInfo().isBigEndian()) {
+            print.output() << "Big";
         } else {
-            Formatter fmt(code_output);
-            CoqPrinter print(fmt);
-            ClangPrinter cprint(compiler_, ctxt);
+            assert(ctxt->getTargetInfo().isLittleEndian());
+            print.output() << "Little";
+        }
 
-            fmt << "Require Import bedrock.lang.cpp.parser." << fmt::line
-                << fmt::line << "#[local] Open Scope bs_scope." << fmt::line;
-            // << "Import ListNotations." << fmt::line;
+        // TODO I still need to generate the initializer
 
-            fmt << fmt::line
-                << "Definition module : translation_unit := " << fmt::indent
-                << fmt::line << "Eval reduce_translation_unit in decls"
+        print.output() << "." << fmt::outdent << fmt::line;
+    });
+
+    with_open_file(notations_file_, [this, &decl, &mod](Formatter& spec_fmt){
+        auto &ctxt = decl->getASTContext();
+        ClangPrinter cprint(compiler_, &decl->getASTContext());
+        CoqPrinter print(spec_fmt, false);
+        // PrintSpec printer(ctxt);
+
+        NoInclude source(ctxt.getSourceManager());
+
+        // print.output() << "(*" << fmt::line
+        //                << " * Notations extracted from "
+        //                << ctxt.getSourceManager()
+        //                       .getFileEntryForID(
+        //                           ctxt.getSourceManager().getMainFileID())
+        //                       ->getName()
+        //                << fmt::line << " *)" << fmt::line;
+        print.output() << "Require Export bedrock.lang.cpp.parser."
+                       << fmt::line << fmt::line;
+
+        // generate all of the record fields
+        write_globals(mod, print, cprint);
+    });
+
+    with_open_file(templates_file_, [this, &ctxt, &mod](Formatter& fmt){
+        CoqPrinter print(fmt, true);
+        ClangPrinter cprint(compiler_, ctxt);
+
+        fmt << "Require Import bedrock.auto.cpp.templates.mparser." << fmt::line
+            << fmt::line
+            << "#[local] Open Scope bs_scope." << fmt::line;
+
+        fmt << fmt::line
+            << "Definition templates : Mtranslation_unit :="
+            << fmt::indent << fmt::line
+                << "Eval Mreduce_translation_unit in Mtranslation_unit.decls"
                 << fmt::nbsp;
 
-            print.begin_list();
-            for (auto entry : mod.declarations()) {
-                if (cprint.printDecl(entry.first, print))
-                    print.cons();
-            }
-            for (auto decl : mod.definitions()) {
-                if (cprint.printDecl(decl, print))
-                    print.cons();
-            }
-            for (auto entry : mod.asserts()) {
-                if (cprint.printDecl(entry, print))
-                    print.cons();
-            }
-            print.end_list();
-            print.output() << fmt::nbsp;
-            if (ctxt->getTargetInfo().isBigEndian()) {
-                print.output() << "Big";
-            } else {
-                assert(ctxt->getTargetInfo().isLittleEndian());
-                print.output() << "Little";
-            }
-
-            // TODO I still need to generate the initializer
-
-            print.output() << "." << fmt::outdent << fmt::line;
+        print.begin_list();
+        for (auto decl : mod.template_declarations()) {
+            printDecl(decl, print, cprint);
         }
-    }
-
-    if (notations_file_.hasValue()) {
-        std::error_code ec;
-        llvm::raw_fd_ostream notations_output(*notations_file_, ec);
-        if (ec.value()) {
-            llvm::errs() << "Failed to open notations file: "
-                         << *notations_file_ << "\n"
-                         << ec.message() << "\n";
-        } else {
-            fmt::Formatter spec_fmt(notations_output);
-            auto &ctxt = decl->getASTContext();
-            ClangPrinter cprint(compiler_, &decl->getASTContext());
-            CoqPrinter print(spec_fmt);
-            // PrintSpec printer(ctxt);
-
-            NoInclude source(ctxt.getSourceManager());
-
-            // print.output() << "(*" << fmt::line
-            //                << " * Notations extracted from "
-            //                << ctxt.getSourceManager()
-            //                       .getFileEntryForID(
-            //                           ctxt.getSourceManager().getMainFileID())
-            //                       ->getName()
-            //                << fmt::line << " *)" << fmt::line;
-            print.output() << "Require Export bedrock.lang.cpp.parser."
-                           << fmt::line << fmt::line;
-
-            // generate all of the record fields
-            write_globals(mod, print, cprint);
+        for (auto decl : mod.template_definitions()) {
+            printDecl(decl, print, cprint);
         }
-    }
+        print.end_list();
+
+        print.output() << "." << fmt::outdent << fmt::line;
+    });
 }
