theories/lang/cpp/parser.v
@@ -6,11 +6,50 @@
 Require Export bedrock.prelude.base.
 Require Export bedrock.lang.cpp.ast.
 
-(** Unsupported types.
-    [description] is meant to be only used for documentation.
- *)
-Definition Tunsupported (description : bs) : type.
-Proof. exact inhabitant. Qed.
+(** * Derived forms used by cpp2v *)
+
+(**
+TODO: Most definitions in this file exists for use in cpp2v-generated
+code where they are immediately reduced away. They could be tucked
+into a module that only gets imported by cpp2v-generated files.
+*)
+
+(** TODO: Misplaced *)
+Fixpoint string_to_bytes (b : bs) : list N :=
+  match b with
+  | BS.EmptyString => nil
+  | BS.String b bs => Byte.to_N b :: string_to_bytes bs
+  end.
+
+(** ** Notations *)
+(**
+TODO: These seem misplaced.
+*)
+
+Declare Custom Entry cppglobal.
+
+Declare Scope cpp_scope.
+Delimit Scope cpp_scope with cpp.
+
+Declare Scope cppfield_scope.
+Delimit Scope cppfield_scope with field.
+Bind Scope cppfield_scope with field.
+
+(* XXX This is only parsing to work around Coq misusing it outside
+[cppfield_scope]. See #235. *)
+Notation "` e `" := e (e custom cppglobal at level 200, at level 0,
+  only parsing) : cppfield_scope.
+
+(** Importing [cpp_notation] makes cpp2v-generated names generally
+available as, e.g., [``::MyClass``]. *)
+Module Export cpp_notation.
+  Notation "'``' e '``'" := e
+    (at level 0, e custom cppglobal at level 200,
+     format "`` e ``") : cpp_scope.
+  Open Scope cpp_scope.
+End cpp_notation.
+
+(** ** Names *)
 
 Fixpoint do_end (ty : globname) : obj_name :=
   match ty with
@@ -40,129 +79,116 @@ Definition Nanon (ty : globname) : globname :=
 
 Definition Cenum_const (e : globname) (x : ident) : obj_name :=
   e ++ "::" ++ x.
-Definition Eenum_const_at (e : globname) (ety ty : type) : Expr :=
-  Ecast Cintegral (Econst_ref (Gname e) ety) Prvalue ty.
 
 Definition pure_virt (x : obj_name) : obj_name * option obj_name :=
   (x, None).
 Definition impl_virt (x : obj_name) : obj_name * option obj_name :=
   (x, Some x).
 
-Definition Sreturn_void : Stmt := Sreturn None.
-Definition Sreturn_val (e : Expr) : Stmt := Sreturn (Some e).
-Definition Sforeach (range ibegin iend : Stmt)
-  (init : option Stmt) (cond : option Expr) (inc : option Expr)
-  (decl body : Stmt) : Stmt :=
-  Sseq [range; ibegin; iend; Sfor init cond inc
-        (Sseq [decl; body])].
-
-(* Indicate that [underlying] is used to represent alias type [name]. Enums are treated similarly. *)
-Definition Talias (name : globname) {underlying : type} : type :=
-  underlying.
-Definition Tunderlying (enum : type) {underlying : type} : type :=
-  underlying.
-
 Definition mk_overrides (methods : list (obj_name * obj_name)) : list (obj_name * obj_name) := methods.
 
 Definition mk_virtuals (methods : list (obj_name * option obj_name)) : list (obj_name * option obj_name) := methods.
 
-Definition NStop : list ident := nil.
+(** ** Types *)
 
-Fixpoint string_to_bytes (b : bs) : list N :=
-  match b with
-  | BS.EmptyString => nil
-  | BS.String b bs => Byte.to_N b :: string_to_bytes bs
-  end.
+Section type.
+  Context {type : Set}.
 
-Bind Scope Z_scope with Z.
+  (**
+  Unsupported types. [description] is meant to be only used for
+  documentation.
+  *)
+  Definition Tunsupported `{!Inhabited type} (description : bs) : type.
+  Proof. exact inhabitant. Qed.
 
-Declare Custom Entry cppglobal.
+  (*
+  Indicate that [underlying] is used to represent alias type [name].
+  Enums are treated similarly.
+  *)
+  Definition Talias (name : globname) {underlying : type} : type :=
+    underlying.
+  Definition Tunderlying (enum : type) {underlying : type} : type :=
+    underlying.
 
-Declare Scope cppfield_scope.
-Delimit Scope cppfield_scope with field.
-Bind Scope cppfield_scope with field.
-(* XXX This is only parsing to work around Coq misusing it outside
-[cppfield_scope]. See #235. *)
-Notation "` e `" := e (e custom cppglobal at level 200, at level 0,
-  only parsing) : cppfield_scope.
-
-(** Importing [cpp_notation] makes cpp2v-generated names generally
-available as, e.g., [``::MyClass``]. *)
-Module Export cpp_notation.
-  Declare Scope cpp_scope.
-  Delimit Scope cpp_scope with cpp.
-  Notation "'``' e '``'" := e
-    (at level 0, e custom cppglobal at level 200,
-     format "`` e ``") : cpp_scope.
-  Open Scope cpp_scope.
-End cpp_notation.
-
+End type.
 Notation Tdecay_type ty := (Qconst (Tptr ty)) (only parsing).
 Notation Tincomplete_array ty := (Qconst (Tptr ty)) (only parsing).
 Notation Tvariable_array ty e := (Qconst (Tptr ty)) (only parsing).
 
-(** this is the compatibility layer, cpp2v generates these definitions
- *)
+(** ** Expressions *)
+
+Definition Eenum_const_at (e : globname) (ety ty : type) : Expr :=
+  Ecast Cintegral (Econst_ref (Gname e) ety) Prvalue ty.
+
+(** ** Statements *)
+
+Section stmt.
+  Context {type Expr : Set}.
+  #[local] Notation Stmt := (Stmt' type Expr).
+
+  Definition Sreturn_void : Stmt := Sreturn None.
+  Definition Sreturn_val (e : Expr) : Stmt := Sreturn (Some e).
+  Definition Sforeach (range ibegin iend : Stmt)
+      (init : option Stmt) (cond : option Expr) (inc : option Expr)
+      (decl body : Stmt) : Stmt :=
+    Sseq [range; ibegin; iend; Sfor init cond inc (Sseq [decl; body])].
+End stmt.
+
+(** ** Translation units *)
+
 Definition translation_unitK : Type :=
   symbol_table -> type_table -> (symbol_table -> type_table -> translation_unit) -> translation_unit.
 
 (** TODO FM-601 don't ignore this *)
 Definition Dstatic_assert (_ : option bs) (_ : Expr) : translation_unitK :=
-  fun syms tys k => k syms tys.
+  fun syms tys k =>
+  k syms tys.
 
 Definition Dvariable (name : obj_name) (t : type) (init : option Expr) : translation_unitK :=
-  fun syms tys k => k (<[ name := Ovar t init ]> syms) tys.
+  fun syms tys k =>
+  k (<[ name := Ovar t init ]> syms) tys.
 
-Definition Dfunction    (name : obj_name) (f : Func) : translation_unitK :=
-  fun syms tys k => k (<[ name := Ofunction f ]> syms) tys.
-Definition Dmethod    (name : obj_name) (f : Method) : translation_unitK :=
-  fun syms tys k => k (<[ name := Omethod f ]> syms) tys.
-Definition Dconstructor    (name : obj_name) (f : Ctor) : translation_unitK :=
-  fun syms tys k => k (<[ name := Oconstructor f ]> syms) tys.
-Definition Ddestructor    (name : obj_name) (f : Dtor) : translation_unitK :=
-  fun syms tys k => k (<[ name := Odestructor f ]> syms) tys.
+Definition Dfunction (name : obj_name) (f : Func) : translation_unitK :=
+  fun syms tys k =>
+  k (<[ name := Ofunction f ]> syms) tys.
+
+Definition Dmethod (name : obj_name) (f : Method) : translation_unitK :=
+  fun syms tys k =>
+  k (<[ name := Omethod f ]> syms) tys.
+
+Definition Dconstructor (name : obj_name) (f : Ctor) : translation_unitK :=
+  fun syms tys k =>
+  k (<[ name := Oconstructor f ]> syms) tys.
+
+Definition Ddestructor (name : obj_name) (f : Dtor) : translation_unitK :=
+  fun syms tys k =>
+  k (<[ name := Odestructor f ]> syms) tys.
 
 Definition Dunion (name : globname) (o : option Union) : translation_unitK :=
   fun syms tys k =>
-    k syms (<[ name := match o with
-                       | None => Gtype
-                       | Some u => Gunion u
-                       end ]> tys).
+  k syms (<[ name := from_option Gunion Gtype o ]> tys).
+
 Definition Dstruct (name : globname) (o : option Struct) : translation_unitK :=
   fun syms tys k =>
-    k syms (<[ name := match o with
-                       | None => Gtype
-                       | Some u => Gstruct u
-                       end ]> tys).
+  k syms (<[ name := from_option Gstruct Gtype o ]> tys).
 
-(* named enumerations *)
 Definition Denum (name : globname) (t : type) (branches : list ident) : translation_unitK :=
-  fun syms tys k => k syms $ <[ name := Genum t branches ]> tys.
-(*
-    let enum_ty := Tnamed name in
-    let raw_ty :=
-        match t with
-        | None => enum_ty
-        | Some t => t
-        end
-    in
-    k syms (List.fold_left (fun acc '(nm, oe) => <[ Cenum_const name nm := Gconstant enum_ty (Some (Eint oe raw_ty)) ]> acc)
-                           branches
-                           match t with
-                           | Some t => <[ name := Genum t (List.map fst branches) ]> tys
-                           | None => tys
-                           end). *)
-  (* ^ enumerations (the initializers need to be constant expressions) *)
+  fun syms tys k =>
+  k syms $ <[ name := Genum t branches ]> tys.
 
 Definition Denum_constant (name : globname) (t ut : type) (v : N + Z) (init : option Expr) : translation_unitK :=
-  fun syms tys k => k syms $ <[ name := Gconstant t (Some (Ecast Cintegral (match v with
-                                                                         | inl n => Echar n ut
-                                                                         | inr z => Eint z ut
-                                                                         end) Prvalue t)) ]> tys.
-Definition Dtypedef     (name : globname) (t : type) : translation_unitK :=
-  fun syms tys k => k syms $ <[ name := Gtypedef t ]> tys.
+  fun syms tys k =>
+  let v := match v with inl n => Echar n ut | inr z => Eint z ut end in
+  k syms $ <[ name := Gconstant t (Some (Ecast Cintegral v Prvalue t)) ]> tys.
+
+Definition Dtypedef (name : globname) (t : type) : translation_unitK :=
+  fun syms tys k =>
+  k syms $ <[ name := Gtypedef t ]> tys.
+
 Definition Dtype (name : globname) : translation_unitK :=
-  fun syms tys k => k syms $ <[ name := Gtype ]> tys.
+  fun syms tys k =>
+  k syms $ <[ name := Gtype ]> tys.
+
 (* Definition translation_unit_canon (c : translation_unit) : translation_unit := *)
 (*   {| symbols := avl.map_canon c.(symbols) *)
 (*    ; globals := avl.map_canon c.(globals) |}. *)
@@ -174,9 +200,10 @@ Fixpoint decls' (ls : list translation_unitK) : translation_unitK :=
   end.
 
 Definition decls ls (e : endian) : translation_unit :=
-  decls' ls ∅ ∅ (fun a b => {| symbols := avl.map_canon a
-                           ; globals := avl.map_canon b
-                           ; initializer := nil (* FIXME *)
-                           ; byte_order := e |}).
+  decls' ls ∅ ∅ $ fun a b =>
+  {| symbols := avl.map_canon a
+  ; globals := avl.map_canon b
+  ; initializer := nil (* FIXME *)
+  ; byte_order := e |}.
 
 Declare Reduction reduce_translation_unit := vm_compute.
